F_mu_ref_conc/examples/stack/CG_stack.v
@@ -1,4 +1,5 @@
-From iris.proofmode Require Import invariants ghost_ownership tactics.
+From iris.proofmode Require Import tactics.
+From iris.base_logic Require Import namespaces.
 From iris_logrel.F_mu_ref_conc Require Import examples.lock.
 Import uPred.
 
@@ -79,20 +80,20 @@ Section CG_Stack.
   Lemma steps_CG_push E ρ j K st v w :
     nclose specN ⊆ E →
     spec_ctx ρ ★ st ↦ₛ v ★ j ⤇ fill K (App (CG_push (Loc st)) (of_val w))
-    ={E}=> j ⤇ fill K Unit ★ st ↦ₛ FoldV (InjRV (PairV w v)).
+    ⊢ |={E}=> j ⤇ fill K Unit ★ st ↦ₛ FoldV (InjRV (PairV w v)).
   Proof.
     intros HNE. iIntros "[#Hspec [Hx Hj]]". unfold CG_push.
-    iVs (step_rec _ _ j K _ _ _ _ with "[Hj]") as "Hj"; eauto.
+    iMod (step_rec _ _ j K _ _ _ _ with "[Hj]") as "Hj"; eauto.
     asimpl.
-    iVs (step_load _ _ j (K ++ [StoreRCtx (LocV _); FoldCtx;
+    iMod (step_load _ _ j (K ++ [StoreRCtx (LocV _); FoldCtx;
                                    InjRCtx; PairRCtx _])
                     _ _ _ with "[Hj Hx]") as "[Hj Hx]"; eauto.
     rewrite ?fill_app. simpl.
     iFrame "Hspec Hj"; trivial.
     rewrite ?fill_app. simpl.
-    iVs (step_store _ _ j K _ _ _ _ _ with "[Hj Hx]") as "[Hj Hx]"; eauto.
+    iMod (step_store _ _ j K _ _ _ _ _ with "[Hj Hx]") as "[Hj Hx]"; eauto.
     { by iFrame. }
-    iVsIntro. by iFrame.
+    iModIntro. by iFrame.
     Unshelve.
     all: try match goal with |- to_val _ = _ => auto using to_of_val end.
     simpl; by rewrite ?to_of_val.
@@ -135,10 +136,10 @@ Section CG_Stack.
     nclose specN ⊆ E →
     spec_ctx ρ ★ st ↦ₛ v ★ l ↦ₛ (#♭v false)
       ★ j ⤇ fill K (App (CG_locked_push (Loc st) (Loc l)) (of_val w))
-    ={E}=> j ⤇ fill K Unit ★ st ↦ₛ FoldV (InjRV (PairV w v)) ★ l ↦ₛ (#♭v false).
+    ⊢ |={E}=> j ⤇ fill K Unit ★ st ↦ₛ FoldV (InjRV (PairV w v)) ★ l ↦ₛ (#♭v false).
   Proof.
     intros HNE. iIntros "[#Hspec [Hx [Hl Hj]]]". unfold CG_locked_push.
-    iVs (steps_with_lock
+    iMod (steps_with_lock
             _ _ j K _ _ _ _ UnitV _ _ _ with "[Hj Hx Hl]") as "Hj"; last done.
     - iIntros (K') "[#Hspec [Hx Hj]]".
       iApply steps_CG_push; first done. iFrame "Hspec Hj Hx"; trivial.
@@ -176,40 +177,40 @@ Section CG_Stack.
     nclose specN ⊆ E →
     spec_ctx ρ ★ st ↦ₛ FoldV (InjRV (PairV w v)) ★
                j ⤇ fill K (App (CG_pop (Loc st)) Unit)
-      ={E}=> j ⤇ fill K (InjR (of_val w)) ★ st ↦ₛ v.
+      ⊢ |={E}=> j ⤇ fill K (InjR (of_val w)) ★ st ↦ₛ v.
   Proof.
     intros HNE. iIntros "[#Hspec [Hx Hj]]". unfold CG_pop.
-    iVs (step_rec _ _ j K _ _ _ _ with "[Hj]") as "Hj"; eauto.
+    iMod (step_rec _ _ j K _ _ _ _ with "[Hj]") as "Hj"; eauto.
     asimpl.
-    iVs (step_load _ _ j (K ++ [CaseCtx _ _; UnfoldCtx])
+    iMod (step_load _ _ j (K ++ [CaseCtx _ _; UnfoldCtx])
                     _ _ _ with "[Hj Hx]") as "[Hj Hx]"; eauto.
     rewrite ?fill_app. simpl.
     iFrame "Hspec Hj"; trivial.
     rewrite ?fill_app. simpl.
-    iVs (step_Fold  _ _ j (K ++ [CaseCtx _ _])
+    iMod (step_Fold  _ _ j (K ++ [CaseCtx _ _])
                     _ _ _ _ with "[Hj]") as "Hj"; eauto.
     rewrite ?fill_app. simpl.
     iFrame "Hspec Hj"; trivial.
     rewrite ?fill_app. simpl.
-    iVs (step_case_inr _ _ j K _ _ _ _ _ with "[Hj]") as "Hj"; eauto.
+    iMod (step_case_inr _ _ j K _ _ _ _ _ with "[Hj]") as "Hj"; eauto.
     asimpl.
-    iVs (step_snd _ _ j (K ++ [AppRCtx (RecV _); StoreRCtx (LocV _)]) _ _ _ _
+    iMod (step_snd _ _ j (K ++ [AppRCtx (RecV _); StoreRCtx (LocV _)]) _ _ _ _
                    _ _ with "[Hj]") as "Hj"; eauto.
     rewrite ?fill_app. simpl.
     iFrame "Hspec Hj"; trivial.
-    iVs (step_store _ _ j (K ++ [AppRCtx (RecV _)]) _ _ _ _ _ _
+    iMod (step_store _ _ j (K ++ [AppRCtx (RecV _)]) _ _ _ _ _ _
           with "[Hj Hx]") as "[Hj Hx]"; eauto.
     rewrite ?fill_app. simpl.
     iFrame "Hspec Hj"; trivial.
     rewrite ?fill_app. simpl.
-    iVs (step_rec _ _ j K _ _ _ _ with "[Hj]") as "Hj"; eauto.
+    iMod (step_rec _ _ j K _ _ _ _ with "[Hj]") as "Hj"; eauto.
     asimpl.
-    iVs (step_fst _ _ j (K ++ [InjRCtx]) _ _ _ _ _ _
+    iMod (step_fst _ _ j (K ++ [InjRCtx]) _ _ _ _ _ _
           with "[Hj]") as "Hj"; eauto.
     rewrite ?fill_app. simpl.
     iFrame "Hspec Hj"; trivial. asimpl.
     rewrite ?fill_app. simpl.
-    iVsIntro. iFrame "Hj Hx"; trivial.
+    iModIntro. iFrame "Hj Hx"; trivial.
     Unshelve.
     all: try match goal with |- to_val _ = _ => simpl; by rewrite ?to_of_val end.
     all: trivial.
@@ -219,24 +220,24 @@ Section CG_Stack.
     nclose specN ⊆ E →
     spec_ctx ρ ★ st ↦ₛ FoldV (InjLV UnitV) ★
                j ⤇ fill K (App (CG_pop (Loc st)) Unit)
-      ={E}=> j ⤇ fill K (InjL Unit) ★ st ↦ₛ FoldV (InjLV UnitV).
+      ⊢ |={E}=> j ⤇ fill K (InjL Unit) ★ st ↦ₛ FoldV (InjLV UnitV).
   Proof.
     iIntros (HNE) "[#Hspec [Hx Hj]]". unfold CG_pop.
-    iVs (step_rec _ _ j K _ _ _ _ with "[Hj]") as "Hj"; eauto.
+    iMod (step_rec _ _ j K _ _ _ _ with "[Hj]") as "Hj"; eauto.
     asimpl.
-    iVs (step_load _ _ j (K ++ [CaseCtx _ _; UnfoldCtx])
+    iMod (step_load _ _ j (K ++ [CaseCtx _ _; UnfoldCtx])
                     _ _ _ with "[Hj Hx]") as "[Hj Hx]"; eauto.
     rewrite ?fill_app. simpl.
     iFrame "Hspec Hj"; trivial.
     rewrite ?fill_app. simpl.
-    iVs (step_Fold _ _ j (K ++ [CaseCtx _ _])
+    iMod (step_Fold _ _ j (K ++ [CaseCtx _ _])
                     _ _ _ _ with "[Hj]") as "Hj"; eauto.
     rewrite ?fill_app. simpl.
     iFrame "Hspec Hj"; trivial.
     rewrite ?fill_app. simpl.
-    iVs (step_case_inl _ _ j K _ _ _ _ _ with "[Hj]") as "Hj"; eauto.
+    iMod (step_case_inl _ _ j K _ _ _ _ _ with "[Hj]") as "Hj"; eauto.
     asimpl.
-    iVsIntro. iFrame "Hj Hx"; trivial.
+    iModIntro. iFrame "Hj Hx"; trivial.
     Unshelve.
     all: try match goal with |- to_val _ = _ => simpl; by rewrite ?to_of_val end.
     all: trivial.
@@ -279,10 +280,10 @@ Section CG_Stack.
     nclose specN ⊆ E →
     spec_ctx ρ ★ st ↦ₛ FoldV (InjRV (PairV w v)) ★ l ↦ₛ (#♭v false)
                ★ j ⤇ fill K (App (CG_locked_pop (Loc st) (Loc l)) Unit)
-      ={E}=> j ⤇ fill K (InjR (of_val w)) ★ st ↦ₛ v ★ l ↦ₛ (#♭v false).
+      ⊢ |={E}=> j ⤇ fill K (InjR (of_val w)) ★ st ↦ₛ v ★ l ↦ₛ (#♭v false).
   Proof.
     iIntros (HNE) "[#Hspec [Hx [Hl Hj]]]". unfold CG_locked_pop.
-    iVs (steps_with_lock _ _ j K _ _ _ _ (InjRV w) UnitV _ _
+    iMod (steps_with_lock _ _ j K _ _ _ _ (InjRV w) UnitV _ _
           with "[Hj Hx Hl]") as "Hj"; last done.
     - iIntros (K') "[#Hspec [Hx Hj]]".
       iApply steps_CG_pop_suc; first done. iFrame "Hspec Hj Hx"; trivial.
@@ -294,10 +295,10 @@ Section CG_Stack.
     nclose specN ⊆ E →
     spec_ctx ρ ★ st ↦ₛ FoldV (InjLV UnitV) ★ l ↦ₛ (#♭v false)
                ★ j ⤇ fill K (App (CG_locked_pop (Loc st) (Loc l)) Unit)
-      ={E}=> j ⤇ fill K (InjL Unit) ★ st ↦ₛ FoldV (InjLV UnitV) ★ l ↦ₛ (#♭v false).
+      ⊢ |={E}=> j ⤇ fill K (InjL Unit) ★ st ↦ₛ FoldV (InjLV UnitV) ★ l ↦ₛ (#♭v false).
   Proof.
     iIntros (HNE) "[#Hspec [Hx [Hl Hj]]]". unfold CG_locked_pop.
-    iVs (steps_with_lock _ _ j K _ _ _ _ (InjLV UnitV) UnitV _ _
+    iMod (steps_with_lock _ _ j K _ _ _ _ (InjLV UnitV) UnitV _ _
           with "[Hj Hx Hl]") as "Hj"; last done.
     - iIntros (K') "[#Hspec [Hx Hj]] /=".
       iApply steps_CG_pop_fail; first done. iFrame "Hspec Hj Hx"; trivial.
@@ -342,18 +343,18 @@ Section CG_Stack.
     nclose specN ⊆ E →
     spec_ctx ρ ★ st ↦ₛ v ★ l ↦ₛ (#♭v false)
                ★ j ⤇ fill K (App (CG_snap (Loc st) (Loc l)) Unit)
-      ={E}=> j ⤇ (fill K (of_val v)) ★ st ↦ₛ v ★ l ↦ₛ (#♭v false).
+      ⊢ |={E}=> j ⤇ (fill K (of_val v)) ★ st ↦ₛ v ★ l ↦ₛ (#♭v false).
   Proof.
     iIntros (HNE) "[#Hspec [Hx [Hl Hj]]]". unfold CG_snap.
-    iVs (steps_with_lock _ _ j K _ _ _ _ v UnitV _ _
+    iMod (steps_with_lock _ _ j K _ _ _ _ v UnitV _ _
           with "[Hj Hx Hl]") as "Hj"; last done; [|by iFrame "Hspec Hx Hl Hj"].
     iIntros (K') "[#Hspec [Hx Hj]]".
-    iVs (step_rec _ _ j K' _ _ _ _ with "[Hj]") as "Hj"; eauto.
+    iMod (step_rec _ _ j K' _ _ _ _ with "[Hj]") as "Hj"; eauto.
     asimpl.
-    iVs (step_load _ _ j K' _ _ _ _
+    iMod (step_load _ _ j K' _ _ _ _
           with "[Hj Hx]") as "[Hj Hx]"; eauto.
     - by iFrame "Hspec Hj Hx".
-    - iVsIntro. by iFrame "Hj Hx".
+    - iModIntro. by iFrame "Hj Hx".
       Unshelve.
       all: try match goal with |- to_val _ = _ => simpl; by rewrite ?to_of_val end.
       all: trivial.
@@ -408,7 +409,7 @@ Section CG_Stack.
     spec_ctx ρ
              ★ j ⤇ fill K (App (CG_iter (of_val f))
                                (Fold (InjR (Pair (of_val w) (of_val v)))))
-      ={E}=>
+      ⊢ |={E}=>
     j ⤇ fill K
           (App
              (Rec
@@ -417,21 +418,21 @@ Section CG_Stack.
              (App (of_val f) (of_val w))).
   Proof.
     iIntros (HNE) "[#Hspec Hj]". unfold CG_iter.
-    iVs (step_rec _ _ j K _ _ _ _ with "[Hj]") as "Hj"; eauto.
+    iMod (step_rec _ _ j K _ _ _ _ with "[Hj]") as "Hj"; eauto.
     rewrite -CG_iter_folding. Opaque CG_iter. asimpl.
-    iVs (step_Fold _ _ j (K ++ [CaseCtx _ _])
+    iMod (step_Fold _ _ j (K ++ [CaseCtx _ _])
                     _ _ _ with "[Hj]") as "Hj"; eauto.
     rewrite ?fill_app /=.
     iFrame "Hspec Hj"; trivial.
     rewrite ?fill_app. asimpl.
-    iVs (step_case_inr _ _ j K _ _ _ _ _ with "[Hj]") as "Hj"; eauto.
+    iMod (step_case_inr _ _ j K _ _ _ _ _ with "[Hj]") as "Hj"; eauto.
     asimpl.
-    iVs (step_fst _ _ j (K ++ [AppRCtx (RecV _); AppRCtx f]) _ _ _ _
+    iMod (step_fst _ _ j (K ++ [AppRCtx (RecV _); AppRCtx f]) _ _ _ _
                    _ _ with "[Hj]") as "Hj"; eauto.
     rewrite ?fill_app /=.
     iFrame "Hspec Hj"; trivial.
     rewrite ?fill_app. simpl.
-    by iVsIntro.
+    by iModIntro.
     Unshelve.
     all: try match goal with |- to_val _ = _ => simpl; by rewrite ?to_of_val end.
   Qed.
@@ -441,17 +442,17 @@ Section CG_Stack.
   Lemma steps_CG_iter_end E ρ j K f :
     nclose specN ⊆ E →
     spec_ctx ρ ★ j ⤇ fill K (App (CG_iter (of_val f)) (Fold (InjL Unit)))
-      ={E}=> j ⤇ fill K Unit.
+      ⊢ |={E}=> j ⤇ fill K Unit.
   Proof.
     iIntros (HNE) "[#Hspec Hj]". unfold CG_iter.
-    iVs (step_rec _ _ j K _ _ _ _ with "[Hj]") as "Hj"; eauto.
+    iMod (step_rec _ _ j K _ _ _ _ with "[Hj]") as "Hj"; eauto.
     rewrite -CG_iter_folding. Opaque CG_iter. asimpl.
-    iVs (step_Fold _ _ j (K ++ [CaseCtx _ _])
+    iMod (step_Fold _ _ j (K ++ [CaseCtx _ _])
                     _ _ _ with "[Hj]") as "Hj"; eauto.
     rewrite ?fill_app /=.
     iFrame "Hspec Hj"; trivial.
     rewrite ?fill_app. asimpl.
-    iVs (step_case_inl _ _ j K _ _ _ _ _ with "[Hj]") as "Hj"; eauto.
+    iMod (step_case_inl _ _ j K _ _ _ _ _ with "[Hj]") as "Hj"; eauto.
     Unshelve.
     all: try match goal with |- to_val _ = _ => simpl; by rewrite ?to_of_val end.
   Qed.
