F_mu_ref_conc/examples/stack/refinement.v
@@ -1,9 +1,10 @@
-From iris.program_logic Require Import auth.
+From iris.base_logic Require Import auth.
+From iris.program_logic Require Import adequacy ectxi_language.
 From iris_logrel.F_mu_ref_conc Require Import soundness_binary.
 From iris_logrel.F_mu_ref_conc.examples Require Import lock.
 From iris_logrel.F_mu_ref_conc.examples.stack Require Import
   CG_stack FG_stack stack_rules.
-From iris.proofmode Require Import invariants ghost_ownership tactics.
+From iris.proofmode Require Import tactics.
 
 Definition stackN : namespace := nroot .@ "stack".
 
@@ -26,22 +27,22 @@ Section Stack_refinement.
     iApply wp_value; eauto.
     iExists (TLamV _); iFrame "Hj".
     clear j K. iAlways. iIntros (τi) "%". iIntros (j K) "Hj /=".
-    iVs (step_tlam _ _ j K with "[Hj]") as "Hj"; eauto.
+    iMod (step_tlam _ _ j K with "[Hj]") as "Hj"; eauto.
     iApply wp_tlam; iNext.
-    iVs (steps_newlock _ _ j (K ++ [AppRCtx (RecV _)]) _ with "[Hj]")
+    iMod (steps_newlock _ _ j (K ++ [AppRCtx (RecV _)]) _ with "[Hj]")
       as (l) "[Hj Hl]"; eauto.
     { rewrite fill_app; simpl. iFrame "Hspec Hj"; trivial. }
     rewrite fill_app; simpl.
-    iVs (step_rec _ _ j K _ _ _ _ with "[Hj]") as "Hj"; eauto.
+    iMod (step_rec _ _ j K _ _ _ _ with "[Hj]") as "Hj"; eauto.
     simpl.
     rewrite CG_locked_push_subst CG_locked_pop_subst
             CG_iter_subst CG_snap_subst. simpl. asimpl.
-    iVs (step_alloc  _ _ j (K ++ [AppRCtx (RecV _)]) _ _ _ _ with "[Hj]")
+    iMod (step_alloc  _ _ j (K ++ [AppRCtx (RecV _)]) _ _ _ _ with "[Hj]")
       as (stk') "[Hj Hstk']"; eauto.
     rewrite fill_app; simpl.
     iFrame "Hspec Hj"; trivial.
     rewrite fill_app; simpl.
-    iVs (step_rec _ _ j K _ _ _ _ with "[Hj]") as "Hj"; eauto.
+    iMod (step_rec _ _ j K _ _ _ _ with "[Hj]") as "Hj"; eauto.
     simpl.
     rewrite CG_locked_push_subst CG_locked_pop_subst
             CG_iter_subst CG_snap_subst. simpl. asimpl.
@@ -50,21 +51,21 @@ Section Stack_refinement.
     all: trivial.
     iApply (wp_bind [AppRCtx (RecV _); AllocCtx; FoldCtx]);
       iApply wp_wand_l; iSplitR; [iIntros (v) "Hv"; iExact "Hv"|].
-    iApply wp_alloc; trivial; iFrame "Hheap"; iNext; iIntros (istk) "Histk".
-    iVsIntro. iApply (wp_bind [AppRCtx (RecV _)]);
+    iApply (wp_alloc with "[]"); trivial; iFrame "#"; iNext; iIntros (istk) "Histk".
+    iApply (wp_bind [AppRCtx (RecV _)]);
       iApply wp_wand_l; iSplitR; [iIntros (v) "Hv"; iExact "Hv"|].
-    iApply wp_alloc; trivial; iFrame "Hheap"; iNext; iIntros (stk) "Hstk".
+    iApply (wp_alloc with "[]"); trivial; iFrame "#"; iNext; iIntros (stk) "Hstk".
     simpl. iApply wp_rec; trivial. iNext. simpl.
     rewrite FG_push_subst FG_pop_subst FG_iter_subst. simpl. asimpl.
     (* establishing the invariant *)
-    iVs (own_alloc (● (∅ : stackUR))) as (γ) "Hemp"; first done.
+    iMod (own_alloc (● (∅ : stackUR))) as (γ) "Hemp"; first done.
     set (istkG := StackG _ _ γ).
     change γ with (@stack_name _ istkG).
     change H0 with (@stack_inG _ istkG).
     clearbody istkG. clear γ H0.
     iAssert (@stack_owns _ istkG _ ∅) with "[Hemp]" as "Hoe".
     { rewrite /stack_owns big_sepM_empty. iFrame "Hemp"; trivial. }
-    iVs (stack_owns_alloc ⊤ _ _ _ with "[Hoe Histk]") as "[Hoe Hls]".
+    iMod (stack_owns_alloc ⊤ _ _ _ with "[Hoe Histk]") as "[Hoe Hls]".
     { by iFrame "Hoe Histk". }
     iAssert (StackLink τi (LocV istk, FoldV (InjLV UnitV))) with "[Hls]" as "HLK".
     { rewrite StackLink_unfold.
@@ -78,7 +79,7 @@ Section Stack_refinement.
                          ★ l ↦ₛ (#♭v false)
              )%I) with "[Hoe Hstk Hstk' HLK Hl]" as "Hinv".
     { iExists _, _, _. by iFrame "Hoe Hstk' Hstk Hl HLK". }
-    iVs (inv_alloc stackN with "[Hinv]") as "#Hinv"; trivial.
+    iMod (inv_alloc stackN with "[Hinv]") as "#Hinv"; trivial.
     { iNext; iExact "Hinv". }
     clear istk.
     Opaque stack_owns.
@@ -102,9 +103,9 @@ Section Stack_refinement.
         iApply (wp_bind [AppRCtx (RecV _)]);
           iApply wp_wand_l; iSplitR; [iIntros (v) "Hv"; iExact "Hv"|].
         iInv stackN as (istk v h) "[Hoe [Hstk' [Hstk [HLK Hl]]]]" "Hclose".
-        iApply (wp_load _ _ _ _ _ _).
-        iIntros "{$Hheap $Hstk} !> Hstk !==>".
-        iVs ("Hclose" with "[Hoe Hstk' HLK Hl Hstk]").
+        iApply (wp_load _ _ _ _ _ _ with "[Hstk]"); first iFrame; iFrame "#".
+        iNext. iIntros "Hstk".
+        iMod ("Hclose" with "[Hoe Hstk' HLK Hl Hstk]").
         { iNext. iExists _, _, _; by iFrame "Hoe Hstk' HLK Hl Hstk". }
         clear v h.
         iApply wp_rec; auto using to_of_val.
@@ -112,8 +113,8 @@ Section Stack_refinement.
         iApply (wp_bind [IfCtx _ _; CasRCtx (LocV _) (FoldV (LocV _));
                                 FoldCtx]);
           iApply wp_wand_l; iSplitR; [iIntros (w) "Hw"; iExact "Hw"|].
-        iApply wp_alloc; simpl; trivial; [by rewrite to_of_val|].
-        iFrame "Hheap". iNext. iIntros (ltmp) "Hltmp". iVsIntro.
+        iApply (wp_alloc with "[]"); simpl; trivial; [by rewrite to_of_val|].
+        iNext. iIntros (ltmp) "Hltmp".
         iApply (wp_bind [IfCtx _ _]);
           iApply wp_wand_l; iSplitR; [by iIntros (w) "$"|].
         iInv stackN as (istk2 v h) "[Hoe [Hstk' [Hstk [HLK Hl]]]]" "Hclose".
@@ -121,27 +122,28 @@ Section Stack_refinement.
         destruct (decide (istk = istk2)) as [|Hneq]; subst.
         * (* CAS succeeds *)
           (* In this case, the specification pushes *)
-          iTimeless "Hstk'". iTimeless "Hl".
-          iVs (steps_CG_locked_push _ _ j K _ _ _ _ _ with "[Hj Hl Hstk']")
+          iMod "Hstk'". iMod "Hl".
+          iMod (steps_CG_locked_push _ _ j K _ _ _ _ _ with "[Hj Hl Hstk']")
             as "[Hj [Hstk' Hl]]".
           { rewrite CG_locked_push_of_val. by iFrame "Hspec Hstk' Hj". }
-          iApply (wp_cas_suc _ _ _ _ _ _ _ _ _ _); simpl; trivial.
-          iIntros "{$Hheap $Hstk} !> Hstk !==>".
-          iVs ("Hclose" with "==>[-Hj]").
-          { iVs (stack_owns_alloc with "[Hoe Hltmp]") as "[Hoe Hpt]".
+          iApply (wp_cas_suc _ _ _ _ _ _ _ _ _ _ with "[Hstk]");
+            first iFrame; iFrame "#".
+          iNext. iIntros "Hstk".
+          iMod ("Hclose" with ">[-Hj]").
+          { iMod (stack_owns_alloc with "[Hoe Hltmp]") as "[Hoe Hpt]".
             { by iFrame "Hoe". }
-            iVsIntro. iNext. iExists ltmp, _, _.
+            iModIntro. iNext. iExists ltmp, _, _.
             iFrame "Hoe Hstk' Hstk Hl".
             do 2 rewrite StackLink_unfold.
             rewrite -StackLink_unfold.
             iExists _, _. iSplit; trivial.
             iFrame "Hpt". eauto 10. }
-          iVsIntro.
+          iModIntro.
           iApply wp_if_true. iNext; iApply wp_value; trivial.
           iExists UnitV; eauto.
-        * iApply (wp_cas_fail _ _ _ _ _ _ _ _ _ _ _ _ _); simpl; trivial.
-          iIntros "{$Hheap $Hstk} !> Hstk !==>".
-          iVs ("Hclose" with "[-Hj]").
+        * iApply (wp_cas_fail _ _ _ _ _ _ _ _ _ _ _ _ _ with "[Hstk]");
+            first iFrame; iFrame "#".
+          iNext. iIntros "Hstk". iMod ("Hclose" with "[-Hj]").
           { iNext. iExists _, _, _. by iFrame "Hoe Hstk' Hstk Hl". }
           iApply wp_if_false. iNext. by iApply "Hlat".
       + (* refinement of pop *)
@@ -157,22 +159,22 @@ Section Stack_refinement.
         iApply (wp_bind [AppRCtx (RecV _); UnfoldCtx]);
           iApply wp_wand_l; iSplitR; [iIntros (v) "Hv"; iExact "Hv"|].
         iInv stackN as (istk v h) "[Hoe [Hstk' [Hstk [HLK Hl]]]]" "Hclose".
-        iApply (wp_load _ _ _ _ _ _). iIntros "{$Hheap $Hstk} !> Hstk".
+        iApply (wp_load _ _ _ _ _ _ with "[Hstk]"); first iFrame; iFrame "#".
+        iNext. iIntros "Hstk".
         (* Checking whether the stack is empty *)
         iDestruct (StackLink_dup with "[HLK]") as "[HLK HLK']"; trivial.
         rewrite {2}StackLink_unfold.
         iDestruct "HLK'" as (istk2 w) "[% [Hmpt [[% %]|HLK']]]"; simplify_eq/=.
         * (* The stack is empty *)
-          iVs (steps_CG_locked_pop_fail _ _ _ _ _ _ _ with "[Hj Hstk' Hl]")
+          iMod (steps_CG_locked_pop_fail _ _ _ _ _ _ _ with "[Hj Hstk' Hl]")
             as "[Hj [Hstk' Hl]]".
           { by iFrame "Hspec Hstk' Hl Hj". }
-          iVsIntro.
-          iVs ("Hclose" with "[-Hj Hmpt]").
+          iMod ("Hclose" with "[-Hj Hmpt]").
           { iNext. iExists _, _, _. by iFrame "Hoe Hstk' Hstk Hl". }
           iApply (wp_bind [AppRCtx (RecV _)]);
             iApply wp_wand_l; iSplitR; [iIntros (w) "Hw"; iExact "Hw"|].
           iApply wp_fold; simpl; auto using to_of_val.
-          iNext. iVsIntro. iApply wp_rec; auto using to_of_val. iNext. asimpl.
+          iNext. iModIntro. iApply wp_rec; auto using to_of_val. iNext. asimpl.
           clear h.
           iApply (wp_bind [AppRCtx (RecV _)]);
             iApply wp_wand_l; iSplitR; [iIntros (w) "Hw"; iExact "Hw"|].
@@ -180,8 +182,9 @@ Section Stack_refinement.
           iDestruct (stack_owns_later_open_close with "[Hmpt Hoe]")
             as "[Histk HLoe]".
           { by iFrame "Hmpt". }
-          iApply (wp_load _ _ _ _ _ _). iFrame "Hheap Histk".
-          iIntros "!> Histk !==>". iVs ("Hclose" with "[-Hj]").
+          iApply (wp_load _ _ _ _ _ _ with "[Histk]");
+            first (iFrame "#"; iFrame).
+          iNext. iIntros "Histk". iMod ("Hclose" with "[-Hj]").
           { iNext. iExists _, _, _. iFrame "Hstk' Hstk HLK Hl".
             iDestruct ("HLoe" with "[Histk]") as "[Hh _]"; trivial.
           }
@@ -191,7 +194,7 @@ Section Stack_refinement.
           iNext. iApply wp_value; simpl; trivial. iExists (InjLV UnitV).
           iSplit; trivial. iLeft. iExists (_, _); repeat iSplit; simpl; trivial.
         * (* The stack is not empty *)
-          iVsIntro. iVs ("Hclose" with "[-Hj Hmpt HLK']").
+          iMod ("Hclose" with "[-Hj Hmpt HLK']").
           { iNext. iExists _, _, _. by iFrame "Hstk' Hstk HLK Hl". }
           iApply (wp_bind [AppRCtx (RecV _)]);
             iApply wp_wand_l; iSplitR; [iIntros (w') "Hw"; iExact "Hw"|].
@@ -204,10 +207,10 @@ Section Stack_refinement.
           iDestruct (stack_owns_later_open_close with "[Hmpt Hoe]")
             as "[Histk HLoe]".
           { by iFrame "Hmpt". }
-          iApply (wp_load _ _ _ _ _ _). iFrame "Hheap Histk".
-          iIntros "!> Histk !==>".
+          iApply (wp_load _ _ _ _ _ _ with "[Histk]"). iFrame "#"; iFrame.
+          iNext; iIntros "Histk".
           iDestruct ("HLoe" with "[Histk]") as "[Hh Hmpt]"; trivial.
-          iVs ("Hclose" with "[-Hj Hmpt HLK']").
+          iMod ("Hclose" with "[-Hj Hmpt HLK']").
           { iNext. iExists _, _, _. by iFrame "Hstk' Hstk HLK Hl". }
           iApply wp_rec; auto using to_of_val.
           iNext. asimpl.
@@ -218,7 +221,7 @@ Section Stack_refinement.
             iApply wp_wand_l; iSplitR; [iIntros (w) "Hw"; iExact "Hw"|].
           asimpl. iApply wp_snd; [simpl; by rewrite ?to_of_val |
                                   simpl; by rewrite ?to_of_val |].
-          simpl. iNext. iVsIntro.
+          simpl. iNext. iModIntro.
           iApply (wp_bind [IfCtx _ _]);
             iApply wp_wand_l; iSplitR; [iIntros (w) "Hw"; iExact "Hw"|].
           clear istk3 h. asimpl.
@@ -227,8 +230,9 @@ Section Stack_refinement.
           destruct (decide (istk2 = istk3)) as [|Hneq]; subst.
           -- (* CAS succeeds *)
             (* In this case, the specification pushes *)
-            iApply (wp_cas_suc _ _ _ _ _ _ _ _ _ _).
-            iIntros "{$Hheap $Hstk} !> Hstk {HLK'}".
+            iApply (wp_cas_suc _ _ _ _ _ _ _ _ _ _ with "[Hstk]");
+              first (iFrame; iFrame "#").
+            iNext. iIntros "Hstk {HLK'}".
             iDestruct (StackLink_dup with "[HLK]") as "[HLK HLK']"; trivial.
             rewrite {2}StackLink_unfold.
             iDestruct "HLK'" as (istk4 w2) "[% [Hmpt' HLK']]"; simplify_eq/=.
@@ -240,11 +244,11 @@ Section Stack_refinement.
                                    "[% [% [#Hrel HLK'']]]"; simplify_eq/=.
              (* Now we have proven that specification can also pop. *)
              rewrite CG_locked_pop_of_val.
-             iVs (steps_CG_locked_pop_suc _ _ _ _ _ _ _ _ _
+             iMod (steps_CG_locked_pop_suc _ _ _ _ _ _ _ _ _
                    with "[Hj Hstk' Hl]") as "[Hj [Hstk' Hl]]".
              { by iFrame "Hspec Hstk' Hl Hj". }
-             iVsIntro. iVs ("Hclose" with "[-Hj]").
-             { iIntros "{Hmpt Hmpt' HLK} !>". rewrite StackLink_unfold.
+             iMod ("Hclose" with "[-Hj]").
+             { iNext. iIntros "{Hmpt Hmpt' HLK}". rewrite StackLink_unfold.
                iDestruct "HLK''" as (istk5 w2) "[% [Hmpt HLK]]"; simplify_eq/=.
                iExists istk5, _, _. iFrame "Hoe Hstk' Hstk Hl".
                rewrite StackLink_unfold.
@@ -256,19 +260,20 @@ Section Stack_refinement.
                iSplitR; [iIntros (w) "Hw"; iExact "Hw"|].
              iApply wp_fst; [simpl; by rewrite ?to_of_val |
                              simpl; by rewrite ?to_of_val |].
-             iNext. iVsIntro. iApply wp_value; simpl.
+             iNext. iModIntro. iApply wp_value; simpl.
              { by rewrite to_of_val. }
              iExists (InjRV _); iFrame "Hj".
              iRight. iExists (_, _). iSplit; trivial.
           -- (* CAS will fail *)
-            iApply (wp_cas_fail  _ _ _ _ _ _ _ _ _ _ _ _ _).
-            iIntros "{$Hheap $Hstk} !> Hstk !==>". iVs ("Hclose" with "[-Hj]").
+            iApply (wp_cas_fail  _ _ _ _ _ _ _ _ _ _ _ _ _ with "[Hstk]");
+            first (iFrame; iFrame "#"). iNext.
+            iIntros "Hstk". iMod ("Hclose" with "[-Hj]").
             { iNext. iExists _, _, _. by iFrame "Hoe Hstk' Hstk HLK Hl". }
             iApply wp_if_false. iNext. by iApply "Hlat".
     - (* refinement of iter *)
       iAlways. clear j K. iIntros ( [f1 f2] ) "/= #Hfs". iIntros (j K) "Hj".
       iApply wp_rec; auto using to_of_val. iNext.
-      iVs (step_rec _ _ _ _ _ _ _ _ _ with "[Hj]") as "Hj".
+      iMod (step_rec _ _ _ _ _ _ _ _ _ with "[Hj]") as "Hj".
       { by iFrame "Hspec Hj". }
       asimpl. rewrite FG_iter_subst CG_snap_subst CG_iter_subst. asimpl.
       replace (FG_iter (of_val f1)) with (of_val (FG_iterV (of_val f1)))
@@ -278,17 +283,17 @@ Section Stack_refinement.
       iApply (wp_bind [AppRCtx _]); iApply wp_wand_l;
         iSplitR; [iIntros (w) "Hw"; iExact "Hw"|].
       iInv stackN as (istk3 w h) "[Hoe [>Hstk' [>Hstk [HLK >Hl]]]]" "Hclose".
-      iVs (steps_CG_snap _ _ _ (K ++ [AppRCtx _]) _ _ _ _
+      iMod (steps_CG_snap _ _ _ (K ++ [AppRCtx _]) _ _ _ _
             with "[Hstk' Hj Hl]") as "[Hj [Hstk' Hl]]".
       { rewrite ?fill_app. simpl. by iFrame "Hspec Hstk' Hl Hj". }
-      iApply (wp_load _ _ _ _ _ _).
-      iIntros "{$Hheap $Hstk} !> Hstk !==>".
+      iApply (wp_load _ _ _ _ _ _ with "[Hstk]"); first (iFrame; iFrame "#").
+      iNext. iIntros "Hstk".
       iDestruct (StackLink_dup with "HLK") as "[HLK HLK']".
-      iVs ("Hclose" with "[-Hj HLK']").
+      iMod ("Hclose" with "[-Hj HLK']").
       { iNext. iExists _, _, _; by iFrame "Hoe Hstk' Hstk HLK Hl". }
       clear h.
       rewrite ?fill_app /= -FG_iter_folding.
-      iLöb (istk3 w) as "Hlat".
+      iLöb as "Hlat" forall (istk3 w).
       rewrite {2}FG_iter_folding.
       iApply wp_rec; simpl; trivial.
       rewrite -FG_iter_folding. asimpl. rewrite FG_iter_subst.
@@ -296,7 +301,7 @@ Section Stack_refinement.
       iApply (wp_bind [CaseCtx _ _; LoadCtx]); iApply wp_wand_l;
         iSplitR; [iIntros (v) "Hw"; iExact "Hw"|].
       iApply wp_fold; simpl; trivial.
-      iNext. iVsIntro. simpl.
+      iNext. iModIntro. simpl.
       iApply (wp_bind [CaseCtx _ _]); iApply wp_wand_l;
         iSplitR; [iIntros (v) "Hw"; iExact "Hw"|].
       rewrite StackLink_unfold.
@@ -305,22 +310,23 @@ Section Stack_refinement.
       iDestruct (stack_owns_later_open_close with "[Hmpt Hoe]")
             as "[Histk HLoe]".
       { by iFrame "Hmpt". }
-      iApply (wp_load _ _ _ _ _ _). iIntros "{$Hheap $Histk} !> Histk".
+      iApply (wp_load _ _ _ _ _ _ with "[Histk]"); first (iFrame; iFrame "#").
+      iNext. iIntros "Histk".
       iDestruct ("HLoe" with "[Histk]") as "[Hh Hmpt]"; trivial.
       iDestruct "HLK'" as "[[% %]|HLK']"; simplify_eq/=.
       * rewrite CG_iter_of_val.
-        iVs (steps_CG_iter_end _ _ _ _ _ _ with "[Hj]") as "Hj".
+        iMod (steps_CG_iter_end _ _ _ _ _ _ with "[Hj]") as "Hj".
         { by iFrame "Hspec Hj". }
-        iVsIntro. iVs ("Hclose" with "[-Hj]").
+        iMod ("Hclose" with "[-Hj]").
         { iNext. iExists _, _, _. by iFrame "Hh Hstk' Hstk HLK". }
         iApply wp_case_inl; trivial.
         iNext. iApply wp_value; trivial. iExists UnitV; eauto.
       * iDestruct "HLK'" as (yn1 yn2 zn1 zn2)
                               "[% [% [#Hrel HLK'']]]"; simplify_eq/=.
         rewrite CG_iter_of_val.
-        iVs (steps_CG_iter _ _ _ _ _ _ _ _ with "[Hj]") as "Hj".
+        iMod (steps_CG_iter _ _ _ _ _ _ _ _ with "[Hj]") as "Hj".
         { by iFrame "Hspec Hj". }
-        iVsIntro. iVs ("Hclose" with "[-Hj HLK'']").
+        iMod ("Hclose" with "[-Hj HLK'']").
         { iNext. iExists _, _, _. by iFrame "Hh Hstk' Hstk HLK". }
         simpl.
         iApply wp_case_inr; simpl; rewrite ?to_of_val; trivial.
@@ -328,7 +334,7 @@ Section Stack_refinement.
         iNext.
         iApply (wp_bind [AppRCtx (RecV _); AppRCtx _]);
           iApply wp_wand_l; iSplitR; [iIntros (w') "Hw"; iExact "Hw"|].
-        iApply wp_fst; simpl; rewrite ?to_of_val; trivial. iNext. iVsIntro.
+        iApply wp_fst; simpl; rewrite ?to_of_val; trivial. iNext. iModIntro.
         iApply (wp_bind [AppRCtx (RecV _)]);
           iApply wp_wand_l; iSplitR; [iIntros (w') "Hw"; iExact "Hw"|].
         rewrite StackLink_unfold.
@@ -339,11 +345,11 @@ Section Stack_refinement.
         iApply wp_wand_l; iSplitR "Hj"; [|iApply "Hfs"; by iFrame "Hj"].
         iIntros (u) "/="; iDestruct 1 as (z) "[Hj [% %]]".
         rewrite fill_app; simpl. subst. asimpl.
-        iVs (step_rec _ _ _ _ _ _ _ _ _ with "[Hj]") as "Hj".
+        iMod (step_rec _ _ _ _ _ _ _ _ _ with "[Hj]") as "Hj".
         { by iFrame "Hspec Hj". } asimpl. rewrite CG_iter_subst. asimpl.
         replace (CG_iter (of_val f2)) with (of_val (CG_iterV (of_val f2)))
           by (by rewrite CG_iter_of_val).
-        iVs (step_snd _ _ _ (K ++ [AppRCtx _]) _ _ _ _ _ _ _ with "[Hj]")
+        iMod (step_snd _ _ _ (K ++ [AppRCtx _]) _ _ _ _ _ _ _ with "[Hj]")
           as "Hj".
         { rewrite fill_app; simpl. by iFrame "Hspec Hj". }
         rewrite fill_app; simpl.
@@ -373,7 +379,7 @@ Theorem stack_ctx_refinement :
         (TArrow TUnit (TSum TUnit (TVar 0))))
         (TArrow (TArrow (TVar 0) TUnit) TUnit)).
 Proof.
-  set (Σ := #[irisΣ lang; authΣ heapUR; authΣ cfgUR; authΣ stackUR]).
+  set (Σ := #[irisΣ state; authΣ heapUR; authΣ cfgUR; authΣ stackUR]).
   eapply (binary_soundness Σ); eauto using FG_stack_closed, CG_stack_closed.
   intros. apply FG_CG_counter_refinement.
 Qed.
