F_mu_ref_conc/soundness_unary.v
@@ -1,6 +1,8 @@
 From iris_logrel.F_mu_ref_conc Require Export fundamental_unary.
-From iris.proofmode Require Import tactics pviewshifts.
-From iris.program_logic Require Import ownership adequacy auth.
+From iris.proofmode Require Import tactics.
+From iris.program_logic Require Import adequacy.
+From iris.base_logic Require Import auth.
+
 
 Theorem soundness Σ `{irisPreG lang Σ, authG Σ heapUR} e τ e' thp σ σ' :
   (∀ `{heapIG Σ}, log_typed [] e τ) →
@@ -9,9 +11,8 @@ Theorem soundness Σ `{irisPreG lang Σ, authG Σ heapUR} e τ e' thp σ σ' :
 Proof.
   intros Hlog ??. cut (adequate e σ (λ _, True)); first (intros [_ ?]; eauto).
   eapply (wp_adequacy Σ); iIntros (?) "Hσ". rewrite -(empty_env_subst e).
-  iVs (auth_alloc (ownP ∘ of_heap) heapN _ (to_heap σ) with "[Hσ]") as (γ) "[??]".
+  iMod (auth_alloc to_heap ownP heapN _ σ with "[Hσ]") as (γ) "[??]"; auto.
   - auto using to_heap_valid.
-  - rewrite /= (from_to_heap σ); auto.
   - iApply wp_wand_l; iSplitR; [|iApply (Hlog (HeapIG _ _ _ γ))]; eauto.
     iSplit. by rewrite /heapI_ctx. iApply (@interp_env_nil _ (HeapIG _ _ _ γ)).
 Qed.
@@ -21,6 +22,6 @@ Corollary type_soundness e τ e' thp σ σ' :
   rtc step ([e], σ) (thp, σ') → e' ∈ thp →
   is_Some (to_val e') ∨ reducible e' σ'.
 Proof.
-  intros ??. set (Σ := #[irisΣ lang ; authΣ heapUR ]).
+  intros ??. set (Σ := #[irisΣ state ; authΣ heapUR ]).
   eapply (soundness Σ); eauto using fundamental.
 Qed.
