prelude/base.v
@@ -1,6 +1,7 @@
 From iris.algebra Require Export base.
-From iris.algebra Require Import upred.
-From iris.program_logic Require Import weakestpre invariants.
+From iris.base_logic Require Import upred.
+From iris.program_logic Require Import weakestpre.
+From iris.base_logic Require Import invariants.
 From Autosubst Require Export Autosubst.
 Import uPred.
 
