README.md
@@ -5,4 +5,4 @@ This version is known to compile with:
  - Coq 8.5pl1
  - Ssreflect 1.6
  - Autosubst 1.5
- - Iris version https://gitlab.mpi-sws.org/FP/iris-coq/commit/f69cdc8c
+ - Iris version https://gitlab.mpi-sws.org/FP/iris-coq/commit/6cb76aaa
